Delete wrong evasive

Evasive.thy
@@ -217,141 +217,34 @@ text\<open>Now we introduce the definition of evasive Boolean function.
 definition evasive :: "nat => (bool vec => bool) => bool"
   where "evasive n f \<equiv> (height (mk_ifex (vec_to_boolfunc n f) [0..<n])) = n"
 
-(* Uff, I completely misunderstood the 
-"An evasive boolean function will satisfy that the height of a corresponding BDD is equal to the number of its vertices"
-I thought that meant "equal to the number of vertices (=graph-nodes) of the bdd", like this:
- *)
-primrec ifex_vertices where
-"ifex_vertices Falseif = 0" |
-"ifex_vertices Trueif = 0" |
-"ifex_vertices (IF _ t e) = Suc (ifex_vertices t + ifex_vertices e)" 
-fun wrong_evasive where
-"wrong_evasive Falseif = True" |
-"wrong_evasive Trueif = True" |
-"wrong_evasive (IF _ t Falseif) = wrong_evasive t" |
-"wrong_evasive (IF _ t Trueif) = wrong_evasive t" |
-"wrong_evasive (IF _ Falseif e) = wrong_evasive e" |
-"wrong_evasive (IF _ Trueif e) = wrong_evasive e" |
-"wrong_evasive (IF _ (IF _ _ _) (IF _ _ _)) = False"
-lemma height_le_vertices: "height f \<le> ifex_vertices f"
+
+primrec ifex_reduce where
+"ifex_reduce Falseif = Falseif" |
+"ifex_reduce Trueif = Trueif" |
+"ifex_reduce (IF v t e) = (let t = ifex_reduce t; e = ifex_reduce e in (if t = e then t else IF v t e))"
+lemma ifex_reduce[simp,intro!]: "ifex_minimal (ifex_reduce f)"
   by(induction f; simp)
-(* this is what I thought evasive was: *)
-lemma wrong_evasive_alt: "wrong_evasive f = (height f = ifex_vertices f)"
-  by(induction f rule: wrong_evasive.induct; simp add: max_def; metis Suc_n_not_le_n height_le_vertices trans_le_add1 trans_le_add2)
+lemma ifex_reduce_varset: "ifex_var_set (ifex_reduce f) \<subseteq> ifex_var_set f"
+  by(induction f) auto
+lemma ifex_reduce_ordered[intro!]: "ifex_ordered f \<Longrightarrow> ifex_ordered (ifex_reduce f)"
+  using ifex_reduce_varset by(induction f) auto
+lemma ifex_reduce_val[simp]: "val_ifex (ifex_reduce f) = val_ifex f"
+  by(induction f) auto
 
-(* I haven't understood well what evasive means.. essentially, there must be one path through
-the bdd where every variable matters *)
-definition "someifex \<equiv> (IF (0 :: nat) (IF 1 Trueif Falseif) (IF 2 Falseif Trueif))"
-lemma "height someifex = 2" "ro_ifex someifex"
-  by eval eval
-(*
-012 V
-FFF T
-FFT F
-FTF T
-FTT F
-TFF F
-TFT F
-TTF T
-TTT T
-*)
-(* you know what confuses me about evasiveness? The height of a bdd is dependend on the atom order.
-I don't see how it makes sense for a property of a boolean function to depend on some arbitrary ordering of the atoms it uses.
-I can't really demonstrate changing the order, but I can demonstrate that the height changes if we rename an atom. *)
-
-(* bit complicated.. would probably have been easier to just reuse mk_ifex *)
-function ifex_mkro where
-"ifex_mkro Falseif = Falseif" |
-"ifex_mkro Trueif = Trueif" |
-"ifex_mkro (IF v t e) = ifex_ite (IF v Trueif Falseif) (ifex_mkro (restrict t v True)) (ifex_mkro (restrict e v False))"
-  by pat_completeness auto
-termination ifex_mkro
-  by (relation "measure (\<lambda>f. card (ifex_var_set f))", rule wf_measure, unfold in_measure) 
-     (rule psubset_card_mono; simp; metis Un_commute Un_insert_right dual_order.refl insert_subset less_supI1 not_element_restrict psubsetI restrict_variables_subset)+
-lemma finite_psubset_induct_my: "finite A \<Longrightarrow> (\<And>A. finite A \<Longrightarrow> (\<And>B. B \<subset> A \<Longrightarrow> P B) \<Longrightarrow> P A) \<Longrightarrow> P A"
-  (* todo: understand why the original isn't usable.. *)
-  using finite_psubset_induct by blast
-lemma ifex_var_set_restrict_ihhelp:
-  "f = IF v t e \<Longrightarrow> r = t \<or> r = e \<Longrightarrow> ifex_var_set (BDT.restrict r v x) \<subset> ifex_var_set f"
-  using not_element_restrict restrict_variables_subset by fastforce
- 
-lemma ro_ifex_mkro[simp,intro!]: "ro_ifex (ifex_mkro f)"
-proof(induction "ifex_var_set f" arbitrary: f rule: finite_psubset_induct_my)
-  case (2 f)
-  then show ?case
-  proof(cases f)
-    case (IF v t e)
-    have "ro_ifex (ifex_mkro (BDT.restrict t v True))"
-         "ro_ifex (ifex_mkro (BDT.restrict e v False))"
-      by (metis "2.hyps"(2) IF ifex_var_set_restrict_ihhelp)+
-    thus ?thesis 
-      by(force simp del: ifex_ite.simps simp add: IF intro!: minimal_ifex_ite_invar order_ifex_ite_invar)
-  qed simp_all
-qed simp
-
-lemma val_ifex_mkro[simp]: "val_ifex (ifex_mkro f) = val_ifex f"
-proof(induction "ifex_var_set f" arbitrary: f rule: finite_psubset_induct_my)
-  case (2 f)
-  then show ?case
-  proof(cases f)
-    case (IF v t e)
-    have "val_ifex (ifex_mkro (BDT.restrict t v True)) = val_ifex (BDT.restrict t v True)"
-         "val_ifex (ifex_mkro (BDT.restrict e v False)) = val_ifex (BDT.restrict e v False)"
-      by (metis "2.hyps"(2) IF ifex_var_set_restrict_ihhelp)+
-    with IF show ?thesis 
-      apply(simp del: ifex_ite.simps)
-      apply(subst val_ifex_ite_subst; (simp; fail)?)
-      apply(simp add: bf_ite_def)
-      apply(rule ext)
-      apply(simp add: restrict_assignment[symmetric] fun_upd_idem)
-      done
-  qed simp_all
-qed simp
-
-definition "ifex_rename from to f \<equiv> ifex_ite (IF to Trueif Falseif) (ifex_mkro (restrict f from True)) (ifex_mkro (restrict f from False))" 
+definition "ifex_rename from to f \<equiv> ifex_ite (IF to Trueif Falseif) (ifex_reduce (restrict f from True)) (ifex_reduce (restrict f from False))" 
 lemma rename_removes: "a \<noteq> b \<Longrightarrow> a \<notin> ifex_var_set (ifex_rename a b f)"
   apply (auto dest!: ifex_vars_subset simp del: ifex_ite.simps simp add: not_element_restrict ifex_rename_def)
   oops
 
-lemma val_ifex_rename: " val_ifex (ifex_rename a b f) assmt = val_ifex f (assmt(a := assmt b))"
+lemma val_ifex_rename: "ifex_ordered f \<Longrightarrow> val_ifex (ifex_rename a b f) assmt = val_ifex f (assmt(a := assmt b))"
   apply (clarsimp simp del: ifex_ite.simps simp add: not_element_restrict ifex_rename_def)
   apply(subst val_ifex_ite_subst)
      apply(simp;fail)
-    apply(simp add: ro_ifex_mkro;fail)
-   apply(simp add: ro_ifex_mkro;fail)
+    apply (simp add: ifex_reduce_ordered restrict_ifex_ordered_invar; fail)
+   apply (simp add: ifex_reduce_ordered restrict_ifex_ordered_invar; fail)
   apply(simp add: bf_ite_def restrict_assignment[symmetric])
   done
-(* end of complicated stuff *)
 
-(* cant change the order, can rename 0 to 3.
-   result: height changes from 2 to 3
- *)
-lemma "height (ifex_rename 0 3 someifex) = 3" by eval
-value "ifex_rename 0 3 someifex"
-
-
-lemma "ro_ifex (IF (0 :: nat) (If 1 Trueif Falseif) (IF 2 Falseif Trueif))"
-  by eval
-lemma assumes "ro_ifex f" shows "height f \<le> card (ifex_var_set f)"
-proof -
-  have "ro_ifex f \<Longrightarrow> n = height f \<Longrightarrow> n \<le> card (ifex_var_set f)" for n
-  proof(induction n arbitrary: f)
-    case 0
-    then show ?case by(cases f; simp)
-  next
-    case (Suc n)
-    obtain i t e where ite: "f = IF i t e" using Suc.prems(2) by(cases f; simp) 
-    hence "i \<notin> (ifex_var_set t \<union> ifex_var_set e)" using Suc.prems(1) by auto
-    hence sc[simp]: "card (insert i (ifex_var_set t \<union> ifex_var_set e)) = Suc (card (ifex_var_set t \<union> ifex_var_set e))"
-      by simp
-    show ?case using Suc.prems Suc.IH[of t] Suc.IH[of e] unfolding ite
-      apply(cases "height t \<le> height e")
-      subgoal by (simp; meson List.finite_set Un_upper2 card_mono finite_Un order_trans)
-      subgoal by (simp; meson List.finite_set card_mono finite_Un order_trans sup_ge1)
-      done
-  qed
-  thus ?thesis using assms by meson
-qed
 
 (*definition evasive :: "nat => ((nat => bool) => bool) => bool"
   where "evasive n f \<equiv> (height (mk_ifex f [0..<n])) = n"*)
@@ -381,28 +274,13 @@ section\<open>The @{term boolean_functions.Alexander_dual} and @{typ "'a ifex"}\
 context boolean_functions
 begin
 
-                           
-(* I don't really see why this should hold without the this_doesnt_hold *)
-lemma 
-  assumes "monotone_bool_fun f"
-  assumes this_doesnt_hold: "vec_to_boolfunc n f = vec_to_boolfunc n (Alexander_dual f)"
-  shows "mk_ifex (vec_to_boolfunc n f) [0..<n] 
-        = mk_ifex (vec_to_boolfunc n (Alexander_dual f)) [0..<n]"
-  using this_doesnt_hold by presburger
-(* If the reason this should hold is somehow hidden in monotone, I lack the insight. *)
-(* Given that the following lemma fails quickcheck, I don't think it is\<dots> *)
-lemma "mono f \<Longrightarrow> (\<not> f (\<lambda>i. \<not> as i)) = f as"
-  oops
-
 primrec ifex_alexander_dual where
 "ifex_alexander_dual Falseif = Trueif" |
 "ifex_alexander_dual Trueif = Falseif" |
 "ifex_alexander_dual (IF i t e) = (IF i (ifex_alexander_dual e) (ifex_alexander_dual t))"
 
-(* Or are you maybe looking for something like this? *)
-lemma "ifex_alexander_dual (mk_ifex (vec_to_boolfunc n f) [0..<n])
+lemma ifex_alexander_dual: "ifex_alexander_dual (mk_ifex (vec_to_boolfunc n f) [0..<n])
   = mk_ifex (vec_to_boolfunc n (Alexander_dual f)) [0..<n]"
-(* but that's trivial, isn't it? *)
 proof -
 
   have ifex_alexander_dual_varset: "ifex_var_set (ifex_alexander_dual f2) = ifex_var_set f2" for f2
